DemoPA.v
@@ -1,0 +1,298 @@
+Require Import FOL.
+Require Import Deduction.
+Require Import Tarski.
+Require Import ProofMode.
+Require Import PA.
+Require Import Equations.Equations Equations.Prop.DepElim.
+Require Import String.
+Require Import List.
+Import ListNotations.
+
+Open Scope string_scope.
+
+
+Section FullLogic.
+Variable p : peirce.
+
+
+(** Setup *)
+
+Ltac custom_fold ::= fold zero in *.
+Ltac custom_unfold ::= unfold zero in *.
+Ltac custom_simpl ::= try rewrite !numeral_subst_invariance.
+
+
+
+
+(** Proof mode and tactics demo *)
+
+Goal forall a b c, nil ⊢ (a --> (a --> b) --> (b --> c) --> c).
+Proof.
+  intros. fstart. fintros. fapply "H1". fapply "H0". fapply "H".
+Qed.
+
+Lemma num_add_homomorphism x y :
+  FA ⊢ (num x ⊕ num y == num (x + y)).
+Proof.
+  induction x; cbn.
+  - fapply ax_add_zero. (* Arguments are infered! *)
+  - feapply ax_trans.
+    + fapply ax_add_rec. 
+    + feapply ax_eq_succ. exact IHx.
+Qed.
+
+Lemma num_mult_homomorphism x y : FA ⊢ ( num x ⊗ num y == num (x * y) ).
+Proof.
+  induction x; cbn.
+  - fapply ax_mult_zero.
+  - feapply ax_trans.
+    + feapply ax_trans.
+      * fapply ax_mult_rec.
+      * feapply ax_eq_add. fapply ax_refl. exact IHx.
+    + apply num_add_homomorphism.
+Qed.
+
+
+
+
+(** Setup rewriting *)
+
+Program Instance PA_Leibniz : Leibniz PA_funcs_signature PA_preds_signature.
+Next Obligation. exact Eq. Defined.
+Next Obligation. exact FA. Defined.
+Next Obligation. fintros. fapply ax_sym. ctx. Defined.
+Next Obligation. fintros. fapply ax_sym. ctx. Defined.
+Next Obligation. Admitted.
+Next Obligation. Admitted. 
+
+
+
+
+(* Rewriting allows for more elegant proofs *)
+
+Lemma num_add_homomorphism' x y :
+  FA ⊢ (num x ⊕ num y == num (x + y)).
+Proof.
+  induction x; cbn.
+  - fapply ax_add_zero.
+  - frewrite <- IHx. fapply ax_add_rec.
+Qed.
+
+Lemma num_mult_homomorphism' x y : FA ⊢ ( num x ⊗ num y == num (x * y) ).
+Proof.
+  induction x; cbn.
+  - fapply ax_mult_zero.
+  - frewrite (ax_mult_rec (num x) (num y)). (* Sadly we need to give the arguments. TODO: Extend tactics to work with terms containing evars *)
+    frewrite IHx. apply num_add_homomorphism'.
+Qed.
+
+
+
+
+(* Rewrite under quantors: *)
+
+Goal forall t t', FA ⊢ (t == t') -> FA ⊢ ∀ $0 ⊕ σ t`[↑] == t' ⊕ σ $0.
+Proof.
+  intros. frewrite H. 
+Abort.
+
+Goal forall t t', FA ⊢ (t == t') -> FA ⊢ ∀∃ $0 ⊕ σ t == t'`[↑]`[↑] ⊕ σ $0.
+Proof.
+  intros. frewrite <- H. 
+Abort.
+
+
+
+
+(* Variable names instead of de Bruijn: *)
+
+Goal FA ⊢ ∀ ∀ $1 == $0 --> σ $1 == zero ⊕ σ $0.
+Proof.
+  fstart. fintros x y "H". frewrite "H". frewrite (ax_add_zero (σ y)).
+  fapply ax_refl.
+Qed.
+
+
+
+
+(** Classical logic *)
+
+Goal forall phi, [] ⊢C (phi ∨ (phi --> ⊥)).
+Proof.
+  intro. fstart. fclassical phi.
+  - fleft. fapply "H".
+  - fright. fapply "H".
+Qed.
+
+Goal forall phi, [] ⊢C (((phi --> ⊥) --> ⊥) --> phi).
+Proof.
+  intro. fstart. fintros. fcontradict as "X". fapply "H". fapply "X".
+Qed.
+
+
+
+
+(** Theories *)
+
+Definition TFA phi := phi el FA.
+
+Lemma num_add_homomorphism_T x y :
+  TFA ⊩ (num x ⊕ num y == num (x + y)).
+Proof.
+  induction x; cbn.
+  - fapply ax_add_zero.
+  - fstart. frewrite <- IHx. fapply ax_add_rec.
+Qed.
+
+Definition TFA_ind : theory := fun phi => phi el FA \/ exists psi, phi = PA_induction psi.
+
+Lemma add_zero_right :
+  TFA_ind ⊩ ∀ $0 ⊕ zero == $0.
+Proof.
+  fstart. assert (TFA_ind ⊩ PA_induction ($0 ⊕ zero == $0)) as H.
+  { apply Ctx. right. now eexists. }
+  unfold PA_induction in H. fapply H; clear H.
+  - fapply ax_add_zero.
+  - fassert ax_trans as "trans". ctx.
+    fassert ax_add_rec as "add_rec". ctx.
+    fassert ax_eq_succ as "eq_succ". ctx.
+    fintros x "IH". feapply "trans".
+    + fapply "add_rec".
+    + fapply "eq_succ". fapply "IH".
+Qed.
+
+
+
+
+(* XM for closed, quantor free formulas: *)
+
+Lemma eq_num t :
+  bound_term 0 t = true -> exists n, FA ⊢ (t == num n).
+Proof.
+  intros H0. induction t.
+  - now exfalso.
+  - destruct F; repeat depelim v; cbn in H0.
+    + exists 0. fapply ax_refl.
+    + destruct (IH h) as [n H]. left. now destruct (bound_term 0 h).
+      exists (S n). cbn. now fapply ax_eq_succ.
+    + destruct (IH h) as [n1 H1]. left. now destruct (bound_term 0 h).
+      destruct (IH h0) as [n2 H2]. right. left. now do 2 destruct bound_term.
+      exists (n1 + n2). assert (H := num_add_homomorphism n1 n2). frewrite <- H.
+      now fapply ax_eq_add.
+    + destruct (IH h) as [n1 H1]. left. now destruct (bound_term 0 h).
+      destruct (IH h0) as [n2 H2]. right. left. now do 2 destruct bound_term.
+      exists (n1 * n2). assert (H := num_mult_homomorphism n1 n2). frewrite <- H.
+      now fapply ax_eq_mult.
+Qed.
+
+Fixpoint quantor_free (phi : form) := match phi with
+| fal => True
+| atom _ _ => True
+| bin _ phi1 phi2 => quantor_free phi1 /\ quantor_free phi2
+| quant _ _ => False
+end.
+
+Lemma xm_quantor_free phi :
+  closed phi = true -> quantor_free phi -> (ax_zero_succ::ax_succ_inj::FA) ⊢ (phi ∨ (phi --> ⊥)).
+Proof.
+  intros H0 H1. induction phi; fstart.
+  - fright. fintros "F". fapply "F".
+  - destruct P. repeat depelim v. cbn in H0, H1. clear H1. 
+    destruct (eq_num h) as [n1 H1]. now destruct bound_term.
+    destruct (eq_num h0) as [n2 H2]. now do 2 destruct bound_term.
+    frewrite H1. frewrite H2. clear H1 H2. 
+    fstop; revert n2; induction n1 as [|n1 IH]; intros; fstart; cbn.
+    + destruct n2; cbn.
+      * fleft. fapply ax_refl.
+      * fright. fapply ax_zero_succ.
+    + destruct n2; cbn.
+      * fright. fintros. feapply ax_zero_succ. feapply ax_sym. ctx.
+      * specialize (IH n2). fdestruct IH as "[IH|IH]".
+        -- fleft. frewrite "IH". fapply ax_refl.
+        -- fright. fintro. fapply "IH". fapply ax_succ_inj. ctx.
+  - cbn in H0, H1. destruct (bound 0 phi1) eqn:H2. 2: now exfalso.
+    fassert (phi1 ∨ (phi1 --> ⊥)) as "IH1" by now fapply IHphi1.
+    fassert (phi2 ∨ (phi2 --> ⊥)) as "IH2" by now fapply IHphi2.
+    destruct b.
+    + fdestruct "IH1" as "[IH1|IH1]". fdestruct "IH2" as "[IH2|IH2]".
+      * fleft. fsplit; ctx.
+      * fright. fintros "[ ]". fapply "IH2". ctx.
+      * fright. fintros "[ ]". fapply "IH1". ctx.
+    + fdestruct "IH1" as "[IH1|IH1]". 2: fdestruct "IH2" as "[IH2|IH2]".
+      * fleft. fleft. ctx.
+      * fleft. fright. ctx.
+      * fright. fintros "[|]". fapply "IH1"; ctx. fapply "IH2"; ctx.
+    + fdestruct "IH1" as "[IH1|IH1]". fdestruct "IH2" as "[IH2|IH2]".
+      * fleft. fintro. ctx.
+      * fright. fintro "H1". fapply "IH2". fapply "H1". ctx.
+      * fleft. fintro. fexfalso. fapply "IH1". ctx.
+  - now exfalso.
+Qed.
+
+
+
+
+(** Attempted Leibniz proof *)
+
+Lemma leibniz_term (t t' s : term) :
+  FA ⊢ (t == t' --> s`[t..] == s`[t'..]).
+Proof.
+  fintros. induction s; cbn.
+  - destruct x; cbn. ctx. fapply ax_refl.
+  - destruct F; repeat depelim v; cbn.
+    * fapply ax_refl.
+    * fapply ax_eq_succ. apply IH. left.
+    * fapply ax_eq_add; apply IH. left. right. left.
+    * fapply ax_eq_mult; apply IH. left. right. left.
+Qed.
+
+Lemma leibniz A phi t t' :
+  FA <<= A -> A ⊢ (t == t') -> A ⊢ phi[t..] -> A ⊢ phi[t'..].
+Proof.
+  intros X. revert t t'. 
+  enough (forall t t', A ⊢ (t == t') -> A ⊢ (phi[t..] --> phi[t'..])) as H0.
+  { intros. specialize (H0 t t' H). fapply (H0 H1). }
+  induction phi; cbn; intros. 1-3: fintros.
+  - ctx.
+  - destruct P. repeat depelim v. cbn in *. feapply ax_trans.
+    + feapply ax_trans. pose (leibniz_term t' t h) as H'. 
+      fapply H'. fapply ax_sym. fapply H. ctx.
+    + pose (leibniz_term t t' h0) as H'. fapply H'. fapply H.
+  - destruct b. 1,2: specialize (IHphi1 t t' H); specialize (IHphi2 t t' H).
+    + fsplit. 
+      * fapply IHphi1. fdestruct 0. ctx. 
+      * fapply IHphi2. fdestruct 0. ctx.
+    + fdestruct 0. 
+      * fleft. fapply IHphi1. ctx.
+      * fright. fapply IHphi2. ctx.
+    + fintros. specialize (IHphi2 t t' H). fapply IHphi2. 
+      fapply 1. assert (A ⊢ (t' == t)) as H' by now fapply ax_sym.
+      specialize (IHphi1 t' t H'). fapply IHphi1. ctx.
+  - destruct q.
+    + 
+Admitted.
+
+
+
+
+(** Division Theorem with Hoas *)
+
+Require Import Hoas.
+
+Lemma division_theorem x y :
+  FA ⊢ << (∃ q r, (∃ k, r ⊕ k == σ bEmbedT (num y)) ∧ bEmbedT (num x) == r ⊕ q ⊗ σ bEmbedT (num y))%hoas.
+Proof.
+  induction x; cbn; fstart.
+  - fexists zero. fexists zero. fsplit.
+    + fexists (σ num y). fapply ax_add_zero.
+    + frewrite (ax_mult_zero (σ num y)). frewrite (ax_add_zero zero).
+      fapply ax_refl.
+  - fdestruct IHx as "[? [? [[? H1] H2]]]".
+    rename x0 into q. rename x1 into r. rename x2 into k.
+    fexists q. fexists (σ r). fsplit.
+    + admit.
+    + frewrite (ax_add_rec (q ⊗ σ num y) r). fapply ax_eq_succ. fapply "H2".
+Abort.
+
+
+
